tests/lean/BaseTutorial.lean
@@ -74,9 +74,9 @@ def mul2_add1 (x : U32) : Result U32 := do
    results explicit.
  -/
 def mul2_add1_desugared (x : U32) : Result U32 :=
-  match Scalar.add x x with
+  match UScalar.add x x with
   | ok x1 => -- Success case
-    match Scalar.add x1 (U32.ofInt 1) with
+    match UScalar.add x1 (U32.ofNat 1) with
     | ok x2 => ok x2
     | error => error
   | error => error -- Propagating the errors
@@ -100,7 +100,7 @@ theorem mul2_add1_spec
      We simply state that [2 * x + 1] must not overflow.
 
      The `.val` notation is used to coerce values. Here, we coerce `x`, which is
-     a bounded machine integer, to an unbounded mathematical integer, which is
+     a bounded machine integer, to an unbounded natural number, which is
      easier to work with. Note that it is also possible to use the `↑x` notation
      to tell Lean to apply a coercion, though Lean may not always be able to figure
      out which coercion to apply (`x.val` is always more precise).
@@ -108,7 +108,7 @@ theorem mul2_add1_spec
   (h : 2 * x.val + 1 ≤ U32.max)
   /- The postcondition -/
   : ∃ y, mul2_add1 x = ok y ∧  -- The call succeeds
-  ↑ y = 2 * ↑x + (1 : Int)   -- The output has the expected value
+  ↑ y = 2 * ↑x + (1 : Nat)   -- The output has the expected value
   := by
   /- The proof -/
   -- Start by a call to the rewriting tactic to reveal the body of [mul2_add1]
@@ -149,12 +149,12 @@ theorem mul2_add1_spec
 
    For this reason, we provide the possibility of registering theorems in a database
    so that [progress] can automatically look them up. This is done by marking
-   theorems with custom attributes, like [pspec] below.
+   theorems with custom attributes, like [progress] below.
 
    Theorems in the standard library like [U32.add_spec] have already been marked with such
    attributes, meaning we don't need to tell [progress] to use them.
  -/
-@[pspec] -- the [pspec] attribute saves the theorem in a database, for [progress] to use it
+@[progress] -- the [progress] attribute saves the theorem in a database, for [progress] to use it
 theorem mul2_add1_spec2 (x : U32) (h : 2 * x.val + 1 ≤ U32.max)
   : ∃ y, mul2_add1 x = ok y ∧
   ↑ y = 2 * ↑x + (1 : Int)
@@ -164,7 +164,7 @@ theorem mul2_add1_spec2 (x : U32) (h : 2 * x.val + 1 ≤ U32.max)
   progress as ⟨ x2 ⟩ -- same
   simp at *; scalar_tac
 
-/- Because we marked [mul2_add1_spec2] theorem with [pspec], [progress] can
+/- Because we marked [mul2_add1_spec2] theorem with [progress], [progress] can
    now automatically look it up. For instance, below:
  -/
 -- A dummy function which uses [mul2_add1]
@@ -172,7 +172,7 @@ def use_mul2_add1 (x : U32) (y : U32) : Result U32 := do
   let x1 ← mul2_add1 x
   x1 + y
 
-@[pspec]
+@[progress]
 theorem use_mul2_add1_spec (x : U32) (y : U32) (h : 2 * x.val + 1 + y.val ≤ U32.max) :
   ∃ z, use_mul2_add1 x y = ok z ∧
   ↑z = 2 * ↑x + (1 : Int) + ↑y := by
@@ -267,7 +267,7 @@ theorem list_nth_spec {T : Type} [Inhabited T] (l : CList T) (i : U32)
   -- Postcondition
   : ∃ x, list_nth T l i = ok x ∧
   -- [x] is the ith element of [l] after conversion to [List]
-  x = l.to_list.index i.toNat
+  x = l.to_list.index i.val
   := by
   -- Here we have to be careful when unfolding the body of [list_nth]: we could
   -- use the [simp] tactic, but it will sometimes loop on recursive definitions.
@@ -280,8 +280,6 @@ theorem list_nth_spec {T : Type} [Inhabited T] (l : CList T) (i : U32)
     -- time [0 ≤ i] (because [i] is a [U32] unsigned integer).
     -- First, let's simplify [to_list CNil] to [0]
     simp [CList.to_list] at h
-    -- Proving we have a contradiction
-    scalar_tac
   | CCons hd tl =>
     -- Simplify the match
     simp only []
@@ -316,7 +314,7 @@ theorem list_nth_spec {T : Type} [Inhabited T] (l : CList T) (i : U32)
       -- by giving it [*] as argument, we tell [simp] to use all the assumptions
       -- to perform rewritings. In particular, it will use [i.val ≠ 0] to
       -- apply [List.index_nzero_cons].
-      have : i.toNat ≠ 0 := by scalar_tac -- Remark: [simp at hi] also works
+      have : i.val ≠ 0 := by scalar_tac -- Remark: [simp at hi] also works
       simp [CList.to_list, *]
 
 /-#===========================================================================#
